LambdaS5/coq/LjsCompleteness.v
@@ -412,7 +412,7 @@ Proof.
     repeat ljs_eval_push.
     unfolds object_props, prop_name.
     simpl in Hopt.
-    match goal with H : binds props _ _ |- _ => 
+    match goal with H : binds (object_properties _) _ _ |- _ => 
         rewrite <- read_option_binds_eq in H; rewrite H in Hopt end.
     solve [false].
     (* set_attr *)
@@ -430,7 +430,7 @@ Proof.
     repeat ljs_eval_push.
     unfolds object_props, prop_name.
     simpl in Hopt.
-    match goal with H : binds props _ _ |- _ => 
+    match goal with H : binds (object_properties _) _ _ |- _ => 
         rewrite <- read_option_binds_eq in H; rewrite H in Hopt end.
     solve [false]. 
     rewrite read_option_binds_eq in Hopt. false. prove_bag.
@@ -450,7 +450,7 @@ Proof.
     unfolds object_extensible. 
     match goal with H : object_oattr_modifiable _ _ |- _ => inverts H end;
     match goal with H : object_oattr_valid _ _ |- _ => inverts H end;
-    simpls; try cases_if; tryfalse; repeat ljs_eval_push.
+    cases_let; substs; try cases_if; simpls; tryfalse; repeat ljs_eval_push.
     (* get_field *)
     unfolds.
     repeat ljs_eval_push.
